issues with sizes of trap handler data

Cheriot/TrapHandler.v
@@ -2,139 +2,107 @@ Require Import Kami.AllNotations ProcKami.Cheriot.InstAssembly ProcKami.Cheriot.
 
 (* Doesn't contain reset code *)
 Section TrapHandler.
-  Variable TimerQuantum: word (Xlen - 1).
-  Variable NumProcesses: word (Xlen / 2).
+  Variable TimerQuantum: word Imm12Sz.
+  Variable NumProcesses: word (Imm12Sz - RegIdSz - 3).
 
   (* MTDC points to trap_handler_data, whose layout is as follows:
    * Cap to Timer (8 bytes)
    * Cap to TimeCmp (8 bytes)
    * Cap to current proc (8 bytes)
-   * proc0 Regs ((NumRegs+1) * 8 bytes)
-   * proc1 Regs ((NumRegs+1) * 8 bytes)
+   * proc0 Regs (NumRegs * 8 bytes)
+   * proc1 Regs (NumRegs * 8 bytes)
    * ...
-   * proc_pred_n Regs ((NumRegs+1) * 8 bytes)
+   * proc_pred_n Regs (NumRegs * 8 bytes)
    *)
   Local Open Scope cheriot_assembly_scope.
 
-  Definition setTimeCmp (mtdcAddr tmp: RegScrName) :=
-    let mTimeAddr := tmp in
-    let mTimeCmpAddr := mtdcAddr in
-    ( clc mTimeAddr, 0#[mtdcAddr] ;;
-      clw tmp, 0#[mTimeAddr] ;;
-      addi tmp, tmp, wordVal _ TimerQuantum ;;
-      clc mTimeCmpAddr, 8#[mtdcAddr] ;;
-      csw 0#[mTimeCmpAddr], tmp
+  Definition getRegIdUnsafe (z: Z) := match getRegNameOpt z with
+                                      | Some name => name
+                                      | None => zero
+                                      end.
+
+  Definition filteredRegsZ (l: list RegScrName) :=
+    filter (fun z: Z => negb (existsb (fun r => Z.eqb z (getRegScrIdZ r)) l)) (map Z.of_nat (seq 1 31)).
+
+  (* curr refers to the register storing the current context cap *)
+  Definition saveAllRegsExcept (curr: RegScrName) (l: list RegScrName) :=
+    fold_right (fun z rest => csc (z * 8)#[curr], (getRegIdUnsafe z) ;; rest) ProgSkip (filteredRegsZ (curr :: l)).
+
+  Definition loadAllRegsExcept (curr: RegScrName) (l: list RegScrName) :=
+    fold_right (fun z rest => clc (getRegIdUnsafe z),  (z * 8)#[curr] ;; rest) ProgSkip (filteredRegsZ (curr :: l)).
+
+  (* curr will finally hold current context in the end *)
+  Definition saveCurrentContext (curr tmp: RegScrName)
+    (pf: isSameRegScr curr tmp = false) :=
+    ( cspecialw mscratchc, curr ;; (* storing current value of curr register into mscratchc *)
+      cspecialr curr, mtdc ;; (* storing mtdc cap into curr register *)
+      clc curr, 16#[curr] ;; (* Current processor offset into curr register, it no longer has mtdc address *)
+      saveAllRegsExcept curr [] ;;
+      cspecialr tmp, mscratchc ;;
+      csc ((getRegScrIdZ curr) * 8)#[curr], tmp ;; (* Store the prev value of curr register, which was in mscratch *)
+      cspecialr tmp, mepcc ;;
+      csc 0#[curr], tmp (* Store mepcc in slot for 0 register of current context *) ).
+
+  Definition mtdcTotalSize := (24 + ((wordVal _ NumProcesses) * ((Z.of_nat NumRegs) * 8)))%Z.
+
+  (* mtdcAddr will contain mtdc cap in the end, curr contains current context in the beginning,
+     curr will contain next context cap in the end *)
+  Definition advanceContext (mtdcAddr curr tmp: RegScrName)
+    (pf1: isSameRegScr mtdcAddr curr = false)
+    (pf2: isSameRegScr curr tmp = false)
+    (pf3: isSameRegScr mtdcAddr tmp = false) :=
+    ( cspecialr mtdcAddr, mtdc ;;
+      cincaddrimm curr, curr, ((Z.of_nat NumRegs) * 8) ;;
+      cincaddrimm tmp, mtdcAddr, mtdcTotalSize ;;
+      LOCAL LSkip;
+      blt curr, tmp, LSkip ;;
+      cincaddrimm curr, mtdcAddr, 24 ;;
+    LSkip :;;
+      csc 16#[mtdcAddr], curr ).
+
+  Definition TimerQuantumZ := wordVal _ TimerQuantum.
+
+  (* mtdcAddr register contains mtdc cap initially, and clobbered in the end *)
+  Definition setTimeCmp (mtdcAddr tmp: RegScrName)
+    (pf: isSameRegScr mtdcAddr tmp = false) :=
+    ( clc tmp, 0#[mtdcAddr] ;;
+      clw tmp, 0#[tmp] ;;
+      addi tmp, tmp, TimerQuantumZ ;;
+      clc mtdcAddr, 8#[mtdcAddr] ;;
+      csw 0#[mtdcAddr], tmp
     ).
 
-  Definition saveRegsFrom2AddrInC1 :=
-    ( csc  16#[c1],  c2 ;;
-      csc  24#[c1],  c3 ;;
-      csc  32#[c1],  c4 ;;
-      csc  40#[c1],  c5 ;;
-      csc  48#[c1],  c6 ;;
-      csc  56#[c1],  c7 ;;
-      csc  64#[c1],  c8 ;;
-      csc  72#[c1],  c9 ;;
-      csc  80#[c1], c10 ;;
-      csc  88#[c1], c11 ;;
-      csc  96#[c1], c12 ;;
-      csc 104#[c1], c13 ;;
-      csc 112#[c1], c14 ;;
-      csc 120#[c1], c15 ;;
-      csc 128#[c1], c16 ;;
-      csc 136#[c1], c17 ;;
-      csc 144#[c1], c18 ;;
-      csc 152#[c1], c19 ;;
-      csc 160#[c1], c20 ;;
-      csc 168#[c1], c21 ;;
-      csc 176#[c1], c22 ;;
-      csc 184#[c1], c23 ;;
-      csc 192#[c1], c24 ;;
-      csc 200#[c1], c25 ;;
-      csc 208#[c1], c26 ;;
-      csc 216#[c1], c27 ;;
-      csc 224#[c1], c28 ;;
-      csc 232#[c1], c29 ;;
-      csc 240#[c1], c30 ;;
-      csc 248#[c1], c31 ).
-
-  (* tmp can be any register except c0/c1 *)
-  Definition saveCurrentContext (tmp: RegScrName) :=
-    ( cspecialw mscratchc, c1 ;;
-      cspecialr c1, mtdc ;;
-      clc c1, 16#[c1] ;;
-      saveRegsFrom2AddrInC1 ;;
-      cspecialr tmp, mepcc ;;
-      csc 0#[c1], tmp ;;
-      cspecialr tmp, mscratchc ;;
-      csc 8#[c1], tmp ;;
-      csrr tmp, mstatus ;;
-      csw 256#[c1], tmp ).
-
-  Definition loadRegsFrom4AddrInC1 :=
-    ( clc  c4,  32#[c1] ;;
-      clc  c5,  40#[c1] ;;
-      clc  c6,  48#[c1] ;;
-      clc  c7,  56#[c1] ;;
-      clc  c8,  64#[c1] ;;
-      clc  c9,  72#[c1] ;;
-      clc c10,  80#[c1] ;;
-      clc c11,  88#[c1] ;;
-      clc c12,  96#[c1] ;;
-      clc c13, 104#[c1] ;;
-      clc c14, 112#[c1] ;;
-      clc c15, 120#[c1] ;;
-      clc c16, 128#[c1] ;;
-      clc c17, 136#[c1] ;;
-      clc c18, 144#[c1] ;;
-      clc c19, 152#[c1] ;;
-      clc c20, 160#[c1] ;;
-      clc c21, 168#[c1] ;;
-      clc c22, 176#[c1] ;;
-      clc c23, 184#[c1] ;;
-      clc c24, 192#[c1] ;;
-      clc c25, 200#[c1] ;;
-      clc c26, 208#[c1] ;;
-      clc c27, 216#[c1] ;;
-      clc c28, 224#[c1] ;;
-      clc c29, 232#[c1] ;;
-      clc c30, 240#[c1] ;;
-      clc c31, 248#[c1] ).
-
-  Definition loadRegsFrom2To3AddrInC1 :=
-    ( clc  c2,  16#[c1] ;;
-      clc  c3,  24#[c1] ).
-
-  (* c1 already contains new context; c2 already contains mtdc; tmp is c3;
-     final regs are based on new context *)
-  Definition loadContextSetTimeCmpMRet :=
-    let mtdcAddr := c2 in
-    let tmp := c3 in
-    ( loadRegsFrom4AddrInC1 ;;
-      setTimeCmp mtdcAddr c3 ;;
-      clw tmp, 256#[c1] ;;
-      csrw mstatus, tmp ;;
-      clc tmp, 0#[c1] ;;
+  (* mtdcAddr contains mtdc cap, curr contains current context cap in the beginning *)
+  Definition loadContextSetTimeCmpMRet (mtdcAddr curr tmp: RegScrName)
+    (pf1: isSameRegScr mtdcAddr curr = false)
+    (pf2: isSameRegScr curr tmp = false)
+    (pf3: isSameRegScr mtdcAddr tmp = false) :=
+    ( loadAllRegsExcept curr [mtdcAddr; tmp] ;;
+      clc tmp, 0#[curr] ;;
       cspecialw mepcc, tmp ;;
-      loadRegsFrom2To3AddrInC1 ;;
-      clc c1, 8#[c1] ;;
+      setTimeCmp mtdcAddr tmp pf3 ;;
+      clc tmp, ((getRegScrIdZ tmp) * 8)#[curr] ;;
+      clc mtdcAddr, ((getRegScrIdZ mtdcAddr) * 8)#[curr] ;;
+      clc curr, ((getRegScrIdZ curr) * 8)#[curr] ;;
       mret ).
 
-  (* mtdcAddr contains mtdc's address finally; c1 contains new context finally;
-     new context is stored in 16#[mtdc] finally; tmp is clobbered *)
-  Definition advanceContext (mtdcAddr tmp: RegScrName) :=
-    ( cspecialr mtdcAddr, mtdc ;;
-      clc c1, 16#[mtdcAddr] ;;
-      cincaddrimm c1, c1, (8*(Z.of_nat NumRegs+1)) ;;
-      cincaddrimm tmp, mtdcAddr, (24+((wordVal _ NumProcesses)*(8*(Z.of_nat NumRegs+1)))) ;;
-      LOCAL LSkip;
-      bge c1, tmp, LSkip ;;
-      cincaddrimm c1, mtdcAddr, 24 ;;
-    LSkip :;;
-      csc 16#[mtdcAddr], c1 ).
+  Definition trapHandler (mtdcAddr curr tmp: RegScrName)
+    (pf1: isSameRegScr mtdcAddr curr = false)
+    (pf2: isSameRegScr curr tmp = false)
+    (pf3: isSameRegScr mtdcAddr tmp = false) :=
+    ( saveCurrentContext curr tmp pf2 ;;
+      advanceContext mtdcAddr curr tmp pf1 pf2 pf3 ;;
+      loadContextSetTimeCmpMRet mtdcAddr curr tmp pf1 pf2 pf3 ).
 
-  Definition trapHandler :=
-    ( saveCurrentContext c2 ;;
-      advanceContext c2 c3 ;;
-      loadContextSetTimeCmpMRet ).
+  (*
+  Definition sizeTrapHandler := match getInstBytes (addi c1, c2, TimerQuantumZ) with
+                                | inl mc => mc
+                                | _ => nil
+                                end.
+
+  Eval compute in sizeTrapHandler.
+  Goal sizeTrapHandler = (4 * 82)%nat.
+    reflexivity.
+  Qed.
+   *)
 End TrapHandler.
